\section{Свойства степени с рациональным показателем}

\begin{theorem}
    \begin{align*}
        &\forall a > 0 \;\; \forall r, q \in \mathbb{Q} \\
        &a^r \cdot a^q = a^{r + q}
    \end{align*}
\end{theorem}

\begin{proof}
    \begin{align*}
        &r, q \in \mathbb{Q} \iff
        \left\{\begin{array}{l}
            m,s \in \mathbb{Z} \\
            n,t \in \mathbb{N} \\
            r = \frac{m}{n} \\
            q = \frac{s}{t}
        \end{array}\right. \Rightarrow
        a^r \cdot a^q = a^\frac{m}{n} \cdot a^\frac{s}{t} = \sqrt[n]{a^m} \cdot \sqrt[t]{a^s} = \sqrt[nt]{a^{mt}} \cdot \sqrt[nt]{a^{sn}} = \\
        &= \sqrt[nt]{a^{mt} \cdot a^{sn}} = \sqrt[nt]{a^{mt + sn}}
        = a^\frac{mt + sn}{nt} = a^{\frac{m}{m} + \frac{s}{t}} = a^{r + q}
    \end{align*}
\end{proof}

\begin{theorem}
    \begin{align*}
        &\forall a > 0 \;\; \forall r, q \in \mathbb{Q} \\
        &a^r : a^q = a^{r - q}
    \end{align*}
\end{theorem}

\begin{proof}
    \begin{align*}
        &r, q \in \mathbb{Q} \iff
        \left\{\begin{array}{l}
            m,s \in \mathbb{Z} \\
            n,t \in \mathbb{N} \\
            r = \frac{m}{n} \\
            q = \frac{s}{t}
        \end{array}\right. \Rightarrow
        a^r : a^q = \frac{a^\frac{m}{n}}{a^\frac{s}{t}} = \frac{\sqrt[n]{a^m}}{\sqrt[t]{a^s}} = \frac{\sqrt[nt]{a^{mt}}}{\sqrt[nt]{a^{sn}}}
        = \sqrt[nt]{\frac{a^{mt}}{a^{sn}}} = \sqrt[nt]{a^{mt - sn}} = a^\frac{mt - sn}{nt} = \\
        &= a^{\frac{m}{n} - \frac{s}{t}} = a^{r - q}
    \end{align*}
\end{proof}

\begin{theorem}
    \begin{align*}
        &\forall a > 0 \;\; \forall r, q \in \mathbb{Q} \\
        &(a^r)^q = a^{rq}
    \end{align*}
\end{theorem}

\begin{proof}
    \begin{align*}
        &r, q \in \mathbb{Q} \iff
        \left\{\begin{array}{l}
            m,s \in \mathbb{Z} \\
            n,t \in \mathbb{N} \\
            r = \frac{m}{n} \\
            q = \frac{s}{t}
        \end{array}\right. \Rightarrow
        (a^r)^q = (a^\frac{m}{n})^\frac{s}{t} = \sqrt[t]{\sqrt[n]{a^m}^s} = \sqrt[nt]{a^{ms}} = a^{\frac{ms}{nt}}
        = a^{\frac{m}{n} \cdot \frac{s}{t}} = a^{rq}
    \end{align*}
\end{proof}

\begin{theorem}
    \begin{align*}
        &\forall a, b > 0 \;\; \forall r \in \mathbb{Q} \\
        &a^r \cdot b^r = (a \cdot b)^r
    \end{align*}
\end{theorem}

\begin{proof}
    \begin{align*}
        &r, q \in \mathbb{Q} \iff
        \left\{\begin{array}{l}
            m \in \mathbb{Z} \\
            n \in \mathbb{N} \\
            r = \frac{m}{n} \\
        \end{array}\right. \Rightarrow
        a^r \cdot b^r = a^\frac{m}{n} \cdot b^\frac{m}{n} = \sqrt[n]{a^m} \cdot \sqrt[n]{b^m} = \sqrt[n]{(a \cdot b)^m} = (ab)^\frac{m}{n}
        = (a \cdot b)^r
    \end{align*}
\end{proof}

\begin{theorem}
    \begin{align*}
        &\forall a, b > 0 \;\; \forall r \in \mathbb{Q} \\
        &\frac{a^r}{b^r}  = \left(\frac{a}{b}\right)^r
    \end{align*}
\end{theorem}

\begin{proof}
    \begin{align*}
        &r, q \in \mathbb{Q} \iff
        \left\{\begin{array}{l}
            m \in \mathbb{Z} \\
            n \in \mathbb{N} \\
            r = \frac{m}{n} \\
        \end{array}\right. \Rightarrow
        \frac{a^r}{b^r} =  \frac{a^\frac{m}{n}}{b^\frac{m}{n}} = \frac{\sqrt[n]{a^m}}{\sqrt[n]{b^m}} = \sqrt[n]{\left(\frac{a}{b}\right)^m}
        =\left(\frac{a}{b}\right)^\frac{m}{n} = \frac{a}{b}^r
    \end{align*}
\end{proof}